SciLean/Core/CoreFunctions.lean
@@ -11,19 +11,130 @@ instance IsLin_is_IsSmooth {X Y : Type} {Xs Y' : Type} [Vec Xs] [Vec Y']
   (n : Nat) (f : X → Y) [Prod.Uncurry n (X → Y) Xs Y'] [inst : IsLinN n f] 
   : IsSmoothN n f := IsSmoothN.mk (toIsSmoothNT:=⟨inst.proof.2⟩)
 
+@[diff] 
+theorem diff_of_linear {X Y} [Vec X] [Vec Y] (f : X → Y) [IsLin f]
+  : ∂ f = λ _ dx => f dx := sorry_proof
 
+@[diff] 
+theorem diff_of_linear_2 {X Y Z} [Vec X] [Vec Y] [Vec Z] (f : X → Y → Z) [IsLinN 2 f]
+  : ∂ (uncurryN 2 f) = λ _ (dx,dy) => f dx dy := sorry_proof
+
+--------------------------------------------------------------------------------
 
 function_properties Neg.neg {X} [Vec X] (x : X) : X
-argument x 
-  isLin := sorry_proof,
+argument x
+  isLin := sorry_proof, 
   isSmooth,
-  abbrev ∂,
-  abbrev 𝒯
+  abbrev ∂ := - dx by symdiff
+  -- abbrev 𝒯 := (-x, -dx) by symdiff
 
 function_properties Neg.neg {X} [SemiHilbert X] (x : X) : X
 argument x
-  hasAdjoint := sorry_proof,
-  abbrev † x' := x' by sorry_proof,
+  hasAdjoint := sorry_proof, 
+  abbrev † := - x' by sorry_proof,
   hasAdjDiff,
-  abbrev ∂†,
-  abbrev ℛ
+  abbrev ∂† := - dx' by unfold adjointDifferential; symdiff; symdiff
+  --abbrev ℛ := (-x, λ dx' => - dx') by symdiff
+
+--------------------------------------------------------------------------------
+
+function_properties HAdd.hAdd {X} [Vec X]  (x y : X) : X
+argument (x,y)
+  isLin := sorry_proof,
+  isSmooth,
+  abbrev ∂ := dx + dy by symdiff
+argument x ..
+  isSmooth := sorry_proof,
+  def ∂ := dx by sorry_proof
+argument y
+  isSmooth := sorry_proof,
+  def ∂ := dy by sorry_proof
+
+function_properties HAdd.hAdd {X} [SemiHilbert X] (x y : X) : X
+argument (x,y)
+  hasAdjoint := sorry_proof,
+  abbrev † := (xy',xy') by sorry_proof,
+  hasAdjDiff := by apply HasAdjDiffN.mk'; symdiff; sorry_proof,
+  abbrev ∂† := (dxy', dxy') by unfold adjointDifferential; symdiff; symdiff
+argument x 
+  hasAdjDiff := sorry_proof,
+  abbrev ∂† := dx' by sorry_proof
+argument y
+  hasAdjDiff := sorry_proof,
+  abbrev ∂† := dy' by sorry_proof
+
+--------------------------------------------------------------------------------
+
+function_properties HSub.hSub {X} [Vec X]  (x y : X) : X
+argument (x,y)
+  isLin := sorry_proof,
+  abbrev ∂ := dx - dy by symdiff
+argument x ..
+  isSmooth := sorry_proof,
+  def ∂ := dx by sorry_proof
+argument y
+  isSmooth := sorry_proof,
+  def ∂ := -dy by sorry_proof
+
+function_properties HSub.hSub {X} [SemiHilbert X] (x y : X) : X
+argument (x,y)
+  hasAdjoint := sorry_proof,
+  hasAdjDiff := by apply HasAdjDiffN.mk'; symdiff; sorry_proof,
+  abbrev † := (xy',-xy') by sorry_proof,
+  abbrev ∂† := (dxy', -dxy') by unfold adjointDifferential; symdiff; symdiff
+argument x 
+  hasAdjDiff := sorry_proof,
+  abbrev ∂† := dx' by sorry_proof
+argument y
+  hasAdjDiff := sorry_proof,
+  abbrev ∂† := -dy' by sorry_proof
+
+--------------------------------------------------------------------------------
+
+function_properties HMul.hMul {X} [Vec X] (x : ℝ) (y : X) : X
+argument (x,y)
+  isSmooth := sorry_proof,
+  abbrev ∂ := dx*y + x*dy by sorry_proof
+argument x ..
+  isLin := sorry_proof, 
+  isSmooth,
+  def ∂ := dx*y by sorry_proof
+argument y
+  isLin := sorry_proof, 
+  isSmooth,
+  def ∂ := x*dy by sorry_proof
+
+function_properties HMul.hMul {X} [SemiHilbert X] (x : ℝ) (y : X) : X
+argument y
+  hasAdjoint := sorry_proof,
+  abbrev † := x*y' by sorry_proof
+  
+function_properties HMul.hMul {X} [Hilbert X] (x : ℝ) (y : X) : X
+argument x
+  hasAdjoint := sorry_proof,
+  abbrev † := ⟪x',y⟫ by sorry_proof
+argument (x,y)
+  hasAdjDiff := by apply HasAdjDiffN.mk'; symdiff; sorry_proof,
+  abbrev ∂† := (⟪dxy',y⟫, x*dxy') by unfold adjointDifferential; symdiff; sorry_proof
+
+--------------------------------------------------------------------------------
+
+function_properties Inner.inner {X} [Hilbert X] (x y : X) : ℝ
+argument (x,y)
+  isSmooth := sorry_proof,
+  abbrev ∂ := ⟪dx,y⟫ + ⟪x,dy⟫ by sorry_proof,
+  hasAdjDiff := by apply HasAdjDiffN.mk'; symdiff; sorry_proof,
+  abbrev ∂† := (dxy'*x, dxy'*y) by sorry_proof
+argument x ..
+  isLin := sorry_proof,
+  isSmooth, 
+  abbrev ∂ := ⟪dx,y⟫ by symdiff
+argument x
+  hasAdjoint := sorry_proof,
+  abbrev † := x'*y by sorry_proof
+argument y
+  isLin := sorry_proof,
+  isSmooth, 
+  abbrev ∂ := ⟪x,dy⟫ by symdiff,
+  hasAdjoint := sorry_proof,
+  abbrev † := y'*x by sorry_proof
