SciLean/Core/FunctionProperties.lean
@@ -1,6 +1,9 @@
+import SciLean.Core.Attributes
 import SciLean.Core.Defs
 import SciLean.Core.Meta.FunctionProperty
 import SciLean.Core.Meta.RewriteBy
+
+import SciLean.Tactic.AutoDiff
 
 namespace SciLean
 
@@ -20,7 +23,7 @@ macro_rules
   let finalCommand ←
     match proof with
     | none =>
-      `(instance (priority:=mid) $instanceId $data.contextBinders* : $instanceType := by first | infer_instance | (unfold $id; apply IsSmoothN.mk); done)
+      `(instance (priority:=mid) $instanceId $data.contextBinders* : $instanceType := by first | infer_instance | apply IsSmoothN.mk | (unfold $id; apply IsSmoothN.mk); done)
     | some proof =>
       `(instance (priority:=mid) $instanceId $data.contextBinders* : $instanceType := $proof)
   
@@ -43,7 +46,7 @@ macro_rules
   let finalCommand ←
     match proof with
     | none =>
-      `(instance (priority:=mid) $instanceId $data.contextBinders* : $instanceType := by unfold $id; apply IsLinN.mk; done)
+      `(instance (priority:=mid) $instanceId $data.contextBinders* : $instanceType := by first | infer_instance | apply IsLinN.mk | (unfold $id; apply IsLinN.mk); done)
     | some proof =>
       `(instance (priority:=mid) $instanceId $data.contextBinders* : $instanceType := $proof)
   
@@ -51,69 +54,225 @@ macro_rules
 
 --------------------------------------------------------------------------------
 
+syntax "hasAdjoint" (":=" term)? : argProp
+
+open Lean Parser.Term in
+macro_rules
+| `(function_property $id:ident $parms:bracketedBinder* $[: $retType:term]? argument $arg:argSpec hasAdjoint $[:= $proof:term]?) => do
+
+  let data ← FunctionPropertyData.parse id parms retType arg
+
+  let instanceId := mkIdent $ data.funPropNamespace.append "hasAdjoint"
+
+  let instanceType ← `(HasAdjointN $data.mainArgNumLit $(← data.mkLambda))
+  let finalCommand ←
+    match proof with
+    | none =>
+      `(instance (priority:=mid) $instanceId $data.contextBinders* : $instanceType := by first | infer_instance | apply HasAdjointN.mk | (unfold $id; apply HasAdjointN.mk); done)
+    | some proof =>
+      `(instance (priority:=mid) $instanceId $data.contextBinders* : $instanceType := $proof)
+  
+  return finalCommand 
+
+--------------------------------------------------------------------------------
+
+theorem HasAdjDiffN.mk' {X Y : Type} {Xs Y' : Type} [SemiHilbert Xs] [SemiHilbert Y']
+  {n : Nat} {f : X → Y} [Prod.Uncurry n (X → Y) Xs Y'] [IsSmoothNT n f]
+  : (∀ x, HasAdjointT $ ∂ (uncurryN n f) x) → HasAdjDiffN n f
+  := λ h => by 
+    have : HasAdjDiffNT n f := by constructor; constructor; infer_instance; apply h
+    apply HasAdjDiffN.mk
+
+syntax "hasAdjDiff" (":=" term)? : argProp
+
+open Lean Parser.Term in
+macro_rules
+| `(function_property $id:ident $parms:bracketedBinder* $[: $retType:term]? argument $arg:argSpec hasAdjDiff $[:= $proof:term]?) => do
+
+  let data ← FunctionPropertyData.parse id parms retType arg
+
+  let instanceId := mkIdent $ data.funPropNamespace.append "hasAdjDiff"
+
+  let instanceType ← `(HasAdjDiffN $data.mainArgNumLit $(← data.mkLambda))
+  let finalCommand ←
+    match proof with
+    | none =>
+      `(instance (priority:=mid) $instanceId $data.contextBinders* : $instanceType := by apply HasAdjDiffN.mk'; symdiff; infer_instance; done)
+    | some proof =>
+      `(instance (priority:=mid) $instanceId $data.contextBinders* : $instanceType := $proof)
+  
+  return finalCommand 
+
+--------------------------------------------------------------------------------
+
+open Lean.Parser.Tactic.Conv
+
 syntax defOrAbbrev := "def" <|> "abbrev"
-syntax termWithProofOrConvTactic := (":=" term "by" term) <|> ("by" term)
+syntax byConvTactic := "by" convSeq
+syntax termAndProof := ":=" term "by" tacticSeq
+syntax termWithProofOrConvTactic := termAndProof <|> byConvTactic
 
 --------------------------------------------------------------------------------
 
 
 syntax defOrAbbrev "∂" (mainArg)? (termWithProofOrConvTactic)? : argProp
 
-
 open Lean Parser.Term in
 macro_rules
-| `(function_property $id:ident $parms:bracketedBinder* $[: $retType:term]? argument $arg:argSpec $a:defOrAbbrev ∂ $[$dargs:mainArg]? $tpc:termWithProofOrConvTactic) => do
+| `(function_property $id:ident $parms:bracketedBinder* $[: $retType:term]? argument $arg:argSpec $doa:defOrAbbrev ∂ $[$dargs:mainArg]? $tpc:termWithProofOrConvTactic) => do
 
   let data ← FunctionPropertyData.parse id parms retType arg 
 
   let lhs := Syntax.mkCApp ``differential #[← data.mkUncurryLambda]
 
   let mainBinder ← data.mainFunBinder
+
   let diffBinder ← 
     match dargs with
     | none => data.mainBinders.mapM (λ b => b.modifyIdent λ ident => mkIdent <| ident.getId.appendBefore "d") 
               >>= mkProdFunBinder
     | some _ => Macro.throwError "Specifying custom names is currently unsupported!"
   let trailingBinders ← data.trailingFunBinders
-  let diffTerm ← 
+
+  let (rhs, proof) ← 
     match tpc with
-    | `(termWithProofOrConvTactic| := $df:term by $proof:term) => pure df
-    | `(termWithProofOrConvTactic| by $conv:term) => default
-    | _ => Macro.throwUnsupported
-  let rhs ← `(λ $mainBinder $diffBinder $trailingBinders* => $diffTerm)
+    | `(termWithProofOrConvTactic| := $df:term by $proof:tacticSeq) =>
+      let rhs ← `(λ $mainBinder $diffBinder $trailingBinders* => $df)
+      let proof ← `(by $proof)
+      pure (rhs, proof)
+
+    | `(termWithProofOrConvTactic| by $c:convSeq) => 
+      let rhs ← `($lhs rewrite_by $c)
+      let proof ← `(by apply AutoImpl.impl_eq_spec)
+      pure (rhs, proof)
+
+    | _ =>  Macro.throwUnsupported
+
+  let definition_name   := mkIdent $ data.funPropNamespace.append "diff"
+  let simp_theorem_name := mkIdent $ data.funPropNamespace.append "diff_simp"
+
+  if doa.raw[0].getAtomVal == "def" then
+    `(
+    def $definition_name $data.contextBinders* := $rhs
+    @[diff] theorem $simp_theorem_name $data.contextBinders* : $lhs = $(data.mkAppContext definition_name) := $proof
+    #print $definition_name
+    #check $simp_theorem_name
+    )
+  else if doa.raw[0].getAtomVal == "abbrev" then
+    `(
+    @[diff] theorem $simp_theorem_name $data.contextBinders* : $lhs = $rhs := $proof
+    #check $simp_theorem_name
+    )
+  else
+    Macro.throwUnsupported
+
+
+--------------------------------------------------------------------------------
+
+
+syntax defOrAbbrev "†" (mainArg)? (termWithProofOrConvTactic)? : argProp
+
+open Lean Parser.Term in
+macro_rules
+| `(function_property $id:ident $parms:bracketedBinder* $[: $retType:term]? argument $arg:argSpec $doa:defOrAbbrev † $[$dargs:mainArg]? $tpc:termWithProofOrConvTactic) => do
+
+  let data ← FunctionPropertyData.parse id parms retType arg 
+
+  let lhs := Syntax.mkCApp ``adjoint #[← data.mkUncurryLambda]
+
+  let mainBinder ← data.mainFunBinder
+
+  let x' := mkIdent s!"{data.mainArgString}'"
+  let adjBinder : TSyntax ``funBinder ← `(($x'))
+
+  let (rhs, proof) ← 
+    match tpc with
+    | `(termWithProofOrConvTactic| := $ft:term by $proof:tacticSeq) =>
+      let mainType ← data.mainArgType
+      let rhs ← `(λ $adjBinder => (($ft) : $mainType))
+      let proof ← `(by $proof)
+      pure (rhs, proof)
+
+    | `(termWithProofOrConvTactic| by $c:convSeq) => 
+      let rhs ← `($lhs rewrite_by $c)
+      let proof ← `(by apply AutoImpl.impl_eq_spec)
+      pure (rhs, proof)
+
+    | _ =>  Macro.throwUnsupported
+
+  let definition_name   := mkIdent $ data.funPropNamespace.append "adjoint"
+  let simp_theorem_name := mkIdent $ data.funPropNamespace.append "adjoint_simp"
+
+  if doa.raw[0].getAtomVal == "def" then
+    `(
+    def $definition_name $data.contextBinders* := $rhs
+    @[diff] theorem $simp_theorem_name $data.contextBinders* : $lhs = $(data.mkAppContext definition_name) := $proof
+    #print $definition_name
+    #check $simp_theorem_name
+    )
+  else if doa.raw[0].getAtomVal == "abbrev" then
+    `(
+    @[diff] theorem $simp_theorem_name $data.contextBinders* : $lhs = $rhs := $proof
+    #check $simp_theorem_name
+    )
+  else
+    Macro.throwUnsupported
+
+--------------------------------------------------------------------------------
+
+
+syntax defOrAbbrev "∂†" (mainArg)? (termWithProofOrConvTactic)? : argProp
+
+open Lean Parser.Term in
+macro_rules
+| `(function_property $id:ident $parms:bracketedBinder* $[: $retType:term]? argument $arg:argSpec $doa:defOrAbbrev ∂† $[$dargs:mainArg]? $tpc:termWithProofOrConvTactic) => do
+
+  let data ← FunctionPropertyData.parse id parms retType arg 
+
+  let lhs := Syntax.mkCApp ``adjointDifferential #[← data.mkUncurryLambda]
+
+  let mainBinder ← data.mainFunBinder
+
+  let x' := mkIdent s!"d{data.mainArgString}'"
+  let adjBinder : TSyntax ``funBinder ← `(($x'))
+
+  dbg_trace (← data.mainArgType).raw.prettyPrint
+
+  let (rhs, proof) ← 
+    match tpc with
+    | `(termWithProofOrConvTactic| := $ft:term by $proof:tacticSeq) =>
+      let mainType ← data.mainArgType
+      let rhs ← `(λ $mainBinder $adjBinder => (($ft) : $mainType))
+      let proof ← `(by $proof)
+      pure (rhs, proof)
+
+    | `(termWithProofOrConvTactic| by $c:convSeq) => 
+      let rhs ← `($lhs rewrite_by $c)
+      let proof ← `(by apply AutoImpl.impl_eq_spec)
+      pure (rhs, proof)
+
+    | _ =>  Macro.throwUnsupported
+
+  let definition_name   := mkIdent $ data.funPropNamespace.append "adjDiff"
+  let simp_theorem_name := mkIdent $ data.funPropNamespace.append "adjDiff_simp"
 
   dbg_trace lhs.raw.prettyPrint
   dbg_trace rhs.raw.prettyPrint
 
-  `(
-    #check $lhs
-    #check $rhs
+  if doa.raw[0].getAtomVal == "def" then
+    `(
+    def $definition_name $data.contextBinders* := $rhs
+    @[diff] theorem $simp_theorem_name $data.contextBinders* : $lhs = $(data.mkAppContext definition_name) := $proof
+    #print $definition_name
+    #check $simp_theorem_name
     )
-  -- let data ← FunctionPropertyData.parse id parms retType arg
+  else if doa.raw[0].getAtomVal == "abbrev" then
+    `(
+    @[diff] theorem $simp_theorem_name $data.contextBinders* : $lhs = $rhs := $proof
+    #check $simp_theorem_name
+    )
+  else
+    Macro.throwUnsupported
 
-  -- let instanceId := mkIdent $ data.funPropNamespace.append "isLin"
 
-  -- let instanceType ← `(IsLinN $data.mainArgNumLit $(← data.mkLambda))
-  -- let finalCommand ←
-  --   match proof with
-  --   | none =>
-  --     `(instance (priority:=mid) $instanceId $data.contextBinders* : $instanceType := by unfold $id; apply IsLinN.mk; done)
-  --   | some proof =>
-  --     `(instance (priority:=mid) $instanceId $data.contextBinders* : $instanceType := $proof)
-  
-  -- return finalCommand 
-
-variable {X} [Vec X]
-
-function_property Neg.neg (x : X) : X
-argument x
-  abbrev ∂ := dx by simp
-
-function_property HAdd.hAdd (x y : X) : X
-argument (x,y)
-  abbrev ∂ := dx + dy by simp
-
-function_property Neg.neg (x : X) : X
-argument x
-  abbrev ∂ by simp
-
+-- variable [SemiHilbert X] [Hilbert X] 
